-- Arian van Putten - 4133935
-- Tim Baanen       - 4134524

module Exercise where

{- Instruction: Fill in all the missing definitions. In most cases,
the type signature enforces that there should be a single unique
definition that fits. 

If you have any questions, don't hesitate to email me or ask in class.
-}


---------------------
------ Prelude ------
---------------------

data ğŸš : Set where
  True : ğŸš
  False : ğŸš

data â„• : Set where
  Zero : â„•
  Succ : â„• â†’ â„•

{-# BUILTIN NATURAL â„• #-}

_+_ : â„• â†’ â„• â†’ â„•
Zero + m = m
Succ k + m = Succ (k + m)

_*_ : â„• â†’ â„• â†’ â„•
Zero * n = Zero
(Succ k) * n = n + (k * n)

data List (a : Set) : Set where
  Nil : List a
  Cons : a â†’ List a â†’ List a

data Vec (a : Set) : â„• â†’ Set where
  Nil : Vec a 0
  Cons : {n : â„•} â†’ (x : a) â†’ (xs : Vec a n) â†’ Vec a (Succ n)

head : {a : Set} {n : â„•} â†’ Vec a (Succ n) â†’ a
head (Cons x xs) = x

append : {a : Set} {n m : â„•} â†’ Vec a n â†’ Vec a m â†’ Vec a (n + m)
append Nil ys = ys
append (Cons x xs) ys = Cons x (append xs ys)

data _â‰¡_ {a : Set} (x : a) : a â†’ Set where
  Refl : x â‰¡ x

cong : {a b : Set} {x y : a} â†’ (f : a â†’ b) â†’ x â‰¡ y â†’ f x â‰¡ f y
cong f Refl = Refl

congâ‚‚ : {a b c : Set} {x y : a} {w z : b} â†’ (f : a â†’ b â†’ c) â†’ x â‰¡ y â†’ w â‰¡ z â†’ f x w â‰¡ f y z
congâ‚‚ f Refl Refl = Refl

data Unit : Set where
  unit : Unit

data Empty : Set where

magic : {a : Set} â†’ Empty â†’ a
magic ()

So : ğŸš -> Set
So True = Unit
So False = Empty

data Pair (a b : Set) : Set where
  _,_ : a â†’ b â†’ Pair a b

data Fin : â„• â†’ Set where
  Fz : âˆ€ {n} â†’ Fin (Succ n)
  Fs : âˆ€ {n} â†’ Fin n â†’ Fin (Succ n)

data Maybe (a : Set) : Set where
  Just : a â†’ Maybe a
  Nothing : Maybe a

-- Casting operator.
the : (a : Set) â†’ a â†’ a
the _ a = a

id : {a : Set} â†’ a â†’ a
id x = x

-- Let's introduce function composition
infixr 25 _âˆ˜_
_âˆ˜_ : {a b c : Set} â†’ (b â†’ c) â†’ (a â†’ b) â†’ (a â†’ c)
(g âˆ˜ f) x = g (f x)

----------------------
----- Exercise 1 -----
----------------------

vmap : {a b : Set} {n : â„•} â†’ (a â†’ b) â†’ Vec a n â†’ Vec b n
vmap f Nil = Nil
vmap f (Cons x xs) = Cons (f x) (vmap f xs)

--- Prove the identity law of functors
vec-functor-id : {n : â„•} {a : Set} â†’  (xs : Vec a n) â†’
  vmap id xs â‰¡ id xs
vec-functor-id Nil = Refl
vec-functor-id (Cons x xs) = cong (Cons x) (vec-functor-id xs)

-- prove that vmap composes (Functor law 2)
vec-functor-comp : âˆ€{a b c g f n} â†’ (xs : Vec a n) â†’
  (vmap g âˆ˜ vmap f) xs â‰¡ vmap (g âˆ˜ f) xs
vec-functor-comp Nil = Refl
vec-functor-comp {g = g} {f} (Cons x xs) =
  cong (Cons ((g âˆ˜ f) x)) (vec-functor-comp xs)

--Show that the Vec a n type is applicative
Î· : {n : â„•} {a : Set} â†’ a â†’ Vec a n
Î· {Zero} a = Nil
Î· {Succ n} a = Cons a (Î· a)

infixl 26 _âŠ™_
_âŠ™_ : {a b : Set} {n : â„•} â†’ Vec (a â†’ b) n â†’ Vec a n â†’ Vec b n
Nil âŠ™ xs = Nil
Cons f vf âŠ™ Cons x xs = Cons (f x) (vf âŠ™ xs)

-- Applicative Identity
vec-app-id : {a : Set } {n : â„•} (v : Vec a n) â†’
  Î· id âŠ™ v â‰¡ v
vec-app-id Nil = Refl
vec-app-id (Cons x v) = cong (Cons (id x)) (vec-app-id v)

-- Applicative Composition
vec-app-comp : {a b c : Set} {n : â„•} (u : Vec (b â†’ c) n) â†’ (v : Vec (a â†’ b) n) â†’ (w : Vec a n) â†’
  (Î· (_âˆ˜_) âŠ™ u âŠ™ v âŠ™ w) â‰¡ u âŠ™ (v âŠ™ w)
vec-app-comp Nil v w = Refl
vec-app-comp (Cons x u) (Cons xâ‚ v) (Cons xâ‚‚ w) = congâ‚‚ Cons Refl (vec-app-comp u v w)

-- Applicative Homomorphism
vec-app-homo : {a b : Set} (n : â„•) â†’ (f : a â†’ b) â†’ (x : a) â†’
  (Î· {n} f) âŠ™ (Î· x) â‰¡ Î· (f x)
vec-app-homo Zero f x = Refl
vec-app-homo (Succ n) f x = cong (Cons (f x)) (vec-app-homo n f x)

-- Applicative Interchange
vec-app-inter : {a b : Set} {y : a} {n : â„•} (u : Vec (a â†’ b) n) â†’
  (u âŠ™ Î· y) â‰¡ (Î· (Î» (f : (a â†’ b)) â†’ f y) âŠ™ u)
vec-app-inter Nil = Refl
vec-app-inter {y = y} (Cons f u) = cong (Cons (f y)) (vec-app-inter u)

----------------------
----- Exercise 2 -----
----------------------

-- Using the Vector definitions, define a type for matrices;
-- matrix addition; the identity matrix; and matrix transposition.

Matrix : Set â†’ â„• â†’ â„• â†’ Set
Matrix a n m = Vec (Vec a n) m

-- Matrix instance for Applicative
mmap : âˆ€ {a b m n} â†’ (a â†’ b) â†’ Matrix a m n â†’ Matrix b m n
mmap f Nil = Nil
mmap f (Cons xs xss) = Cons (vmap f xs) (mmap f xss)

_â“œ_ : âˆ€ {a b m n} â†’ Matrix (a â†’ b) m n â†’ Matrix a m n â†’ Matrix b m n
Nil â“œ Nil = Nil
Cons fs fss â“œ Cons xs xss = Cons (fs âŠ™ xs) (fss â“œ xss)

-- Define matrix addition
madd : {n m : â„•} â†’ Matrix â„• m n â†’ Matrix â„• m n â†’ Matrix â„• m n
madd xss yss = (mmap _+_ xss) â“œ yss

-- Define matrix transposition
transpose : {n m : â„•} {a : Set} â†’ Matrix a m n â†’ Matrix a n m
transpose Nil = Î· Nil
transpose (Cons xs xss) = vmap Cons xs âŠ™ transpose xss

----------------------
----- Exercise 3 -----
----------------------

-- Define a few functions manipulating finite types.

-- The result of "plan {n}" should be a vector of length n storing all
-- the inhabitants of Fin n in increasing order.
plan : {n : â„•} â†’ Vec (Fin n) n
plan {Zero} = Nil
plan {Succ n} = Cons Fz (vmap Fs plan)

-- Define a forgetful map, mapping Fin to â„•
forget : {n : â„•} â†’ Fin n â†’ â„•
forget Fz = Zero
forget (Fs i) = Succ (forget i)

-- There are several ways to embed Fin n in Fin (Succ n).  Try to come
-- up with one that satisfies the correctness property below (and
-- prove that it does).
embed : {n : â„•} â†’ Fin n â†’ Fin (Succ n)
embed Fz = Fz
embed (Fs i) = Fs (embed i)

correct : {n : â„•} â†’ (i : Fin n) â†’ forget i â‰¡ forget (embed i)
correct Fz = Refl
correct (Fs i) = cong Succ (correct i)

----------------------
----- Exercise 4 -----
----------------------

-- Given the following data type definition:

data Compare : â„• â†’ â„• â†’ Set where
  LessThan : âˆ€ {n} k â†’ Compare n (n + Succ k)
  Equal : âˆ€ {n} â†’ Compare n n
  GreaterThan : âˆ€ {n} k â†’ Compare (n + Succ k) n

-- Show that there is a 'covering function'
cmp : (n m : â„•) â†’ Compare n m
cmp Zero Zero = Equal
cmp Zero (Succ m) = LessThan m
cmp (Succ n) Zero = GreaterThan n
cmp (Succ n) (Succ m) with cmp n m
cmp (Succ n) (Succ .(n + Succ k)) | LessThan k = LessThan k
cmp (Succ m) (Succ .m)            | Equal = Equal
cmp (Succ .(m + Succ k)) (Succ m) | GreaterThan k = GreaterThan k

-- Use the cmp function you defined above to define the absolute
-- difference between two natural numbers.
difference : (n m : â„•) â†’ â„•
difference n m  with cmp n m
difference n .(n + Succ k) | LessThan k = Succ k
difference m .m            | Equal = 0
difference .(m + Succ k) m | GreaterThan k = Succ k 

----------------------
----- Exercise 5 -----
----------------------

-- Prove the following equalities.  You may want to define auxiliary
-- lemmas or use the notation intoduced in the lectures.

sym : {a : Set} {x y : a} â†’ x â‰¡ y â†’ y â‰¡ x
sym Refl = Refl

trans : {a : Set} {x y z : a} â†’ x â‰¡ y â†’ y â‰¡ z â†’ x â‰¡ z
trans Refl Refl = Refl

infixr 2 _â‰¡âŸ¨_âŸ©_
_â‰¡âŸ¨_âŸ©_ : {a : Set} â†’ (x : a) â†’ {y z : a} â†’ x â‰¡ y â†’ y â‰¡ z â†’ x â‰¡ z
x â‰¡âŸ¨ p âŸ© q = trans p q

_âˆ : {a : Set} (x : a) â†’ x â‰¡ x
_âˆ x = Refl

plusZero : (n : â„•) â†’ (n + 0) â‰¡ n
plusZero Zero = Refl
plusZero (Succ n) = cong Succ (plusZero n)

plusSucc : (n m : â„•) â†’ Succ (n + m) â‰¡ (n + Succ m)
plusSucc Zero m = Refl
plusSucc (Succ n) m = cong Succ (plusSucc n m)

plusCommutes : (n m : â„•) â†’ (n + m) â‰¡ (m + n)
plusCommutes Zero m = sym (plusZero m)
plusCommutes (Succ n) m =
    ((Succ n) + m)
    â‰¡âŸ¨ cong Succ (plusCommutes n m) âŸ©
    Succ (m + n)
    â‰¡âŸ¨ plusSucc m n âŸ©
    (m + (Succ n))
    âˆ

plusAssociates : (n m k : â„•) â†’ ((n + m) + k) â‰¡ (n + (m + k))
plusAssociates Zero m k = Refl
plusAssociates (Succ n) m k = cong Succ (plusAssociates n m k)

plusDistributes : (n m k l : â„•) â†’ ((n + m) + (k + l)) â‰¡ ((n + k) + (m + l))
plusDistributes n m k l =
    ((n + m) + (k + l))
    â‰¡âŸ¨ plusAssociates n m (k + l) âŸ©
    (n + (m + (k + l)))
    â‰¡âŸ¨ cong (_+_ n) (sym (plusAssociates m k l)) âŸ©
    (n + ((m + k) + l))
    â‰¡âŸ¨ cong (Î» x â†’ n + (x + l)) (plusCommutes m k) âŸ©
    (n + ((k + m) + l))
    â‰¡âŸ¨ cong (_+_ n) (plusAssociates k m l) âŸ©
    (n + (k + (m + l)))
    â‰¡âŸ¨ sym (plusAssociates n k (m + l)) âŸ©
    ((n + k) + (m + l))
    âˆ

distributivity : (n m k : â„•) â†’ (n * (m + k)) â‰¡ ((n * m) + (n * k))
distributivity Zero m k = Refl
distributivity (Succ n) m k =
    ((m + k) + (n * (m + k)))
    â‰¡âŸ¨ cong (_+_ (m + k)) (distributivity n m k) âŸ©
    ((m + k) + ((n * m) + (n * k)))
    â‰¡âŸ¨ plusDistributes m k (n * m) (n * k) âŸ©
    ((m + (n * m)) + (k + (n * k)))
    âˆ

----------------------
----- Exercise 6 -----
----------------------

-- Prove that the sublist relation defined below is transitive and reflexive.

data SubList {a : Set} : List a â†’ List a â†’ Set where
  Base : SubList Nil Nil
  Keep : âˆ€ {x xs ys} â†’ SubList xs ys â†’ SubList (Cons x xs) (Cons x ys)
  Drop : âˆ€ {y zs ys} â†’ SubList zs ys â†’ SubList zs (Cons y ys)

SubListRefl : {a : Set} {xs : List a} â†’ SubList xs xs
SubListRefl {a} {Nil} = Base
SubListRefl {a} {Cons x xs} = Keep SubListRefl

SublistCons : {a : Set} {xs ys : List a} {x : a} â†’ SubList (Cons x xs) ys â†’ SubList xs ys
SublistCons {a} {xs} {Nil} {x} ()
SublistCons {a} {xs} {Cons x ys} {.x} (Keep x<y) = Drop x<y
SublistCons {a} {xs} {Cons xâ‚ ys} {x} (Drop x<y) = Drop (SublistCons x<y)

SubListTrans : {a : Set} {xs ys zs : List a} â†’ SubList xs ys â†’ SubList ys zs â†’ SubList xs zs
SubListTrans Base y<z = y<z
SubListTrans (Keep x<y) (Keep y<z) = Keep (SubListTrans x<y y<z)
SubListTrans (Keep x<y) (Drop y<z) = Drop (SubListTrans (Keep x<y) y<z)
SubListTrans (Drop x<y) (Keep y<z) = Drop (SubListTrans x<y y<z)
SubListTrans (Drop x<y) (Drop y<z) = Drop (SubListTrans x<y (SublistCons y<z))

-- Note that this function doesn't seem to terminate,
-- but since we have to show absurdity, we can't actually terminate!
ConsNotSubList : {a : Set} {xs : List a} {x : a} â†’ SubList (Cons x xs) xs â†’ Empty
ConsNotSubList {a} {Cons x ys} {.x} (Keep xx<x) = ConsNotSubList xx<x
ConsNotSubList {a} {Cons y ys} {x} (Drop xx<x) = ConsNotSubList (SublistCons xx<x)

SubListAntiSym : {a : Set} {xs ys : List a} â†’  SubList xs ys â†’ SubList ys xs â†’ xs â‰¡ ys
SubListAntiSym {a} {.Nil} {.Nil} Base Base = Refl
SubListAntiSym {a} {(Cons x _)} {.(Cons x _)} (Keep x<y) (Keep y<x) = cong (Cons x) (SubListAntiSym x<y y<x)
SubListAntiSym {a} {.(Cons _ _)} {.(Cons _ _)} (Keep x<y) (Drop y<x) = magic (ConsNotSubList (SubListTrans y<x x<y))
SubListAntiSym {a} {xs} {.(Cons _ _)} (Drop x<y) y<x = magic (ConsNotSubList (SubListTrans y<x x<y))

----------------------
----- Exercise 7 -----
----------------------

-- Define the constructors of a data type
data _â‰¤_ : â„• â†’ â„• â†’ Set where
  0â‰¤n : âˆ€ {n} â†’ Zero â‰¤ n
  n+1â‰¤m+1 : âˆ€ {n m} â†’ n â‰¤ m â†’ (Succ n) â‰¤ (Succ m)

-- (Alternative correct definitions exist - this one is the easiest to
-- work with for the rest of this exercise)

â‰¤-refl : (n : â„•) â†’ n â‰¤ n
â‰¤-refl Zero = 0â‰¤n
â‰¤-refl (Succ n) = n+1â‰¤m+1 (â‰¤-refl n)

â‰¤-trans : {n m k : â„•} â†’ n â‰¤ m â†’ m â‰¤ k â†’ n â‰¤ k
â‰¤-trans 0â‰¤n b = 0â‰¤n
â‰¤-trans (n+1â‰¤m+1 a) (n+1â‰¤m+1 b) = n+1â‰¤m+1 (â‰¤-trans a b)

â‰¤-antiSym : {n m : â„•} â†’ n â‰¤ m â†’ m â‰¤ n â†’ n â‰¡ m
â‰¤-antiSym 0â‰¤n 0â‰¤n = Refl
â‰¤-antiSym (n+1â‰¤m+1 a) (n+1â‰¤m+1 b) = cong Succ (â‰¤-antiSym a b)

-- Given the following function:
_â‰¤?_ : â„• â†’ â„• â†’ ğŸš
Zero â‰¤? y = True
Succ x â‰¤? Zero = False
Succ x â‰¤? Succ y = x â‰¤? y

-- Now show that this function behaves as the LEQ data type

soundnessâ‰¤ : {n m : â„•} â†’ n â‰¤ m â†’ So (n â‰¤? m)
soundnessâ‰¤ 0â‰¤n = unit
soundnessâ‰¤ (n+1â‰¤m+1 nâ‰¤m) = soundnessâ‰¤ nâ‰¤m

completenessâ‰¤ : (n m : â„•) â†’ So (n â‰¤? m) â†’ n â‰¤ m
completenessâ‰¤ Zero m nâ‰¤m = 0â‰¤n
completenessâ‰¤ (Succ n) Zero ()
completenessâ‰¤ (Succ n) (Succ m) nâ‰¤m = n+1â‰¤m+1 (completenessâ‰¤ n m nâ‰¤m)

----------------------
----- Exercise 7 -----
----------------------

-- We can define negation as follows
Â¬_ : Set â†’ Set
Â¬ P = P â†’ Empty

-- Agda's logic is *constructive*, meaning some properties you may be
-- familiar with from classical logic do not hold.

notNotP : {P : Set} â†’ P â†’ Â¬ (Â¬ P)
notNotP p notP = notP p

-- The reverse does not hold: Â¬ (Â¬ P) does not imply P

-- Similarly, P or Â¬ P doesn't hold for all statements P, but we can
-- prove the statement below. It's an amusing brainteaser.

data _âˆ¨_ (a b : Set) : Set where
  Inl : a â†’ a âˆ¨ b
  Inr : b â†’ a âˆ¨ b

orCase : {a b c : Set} â†’ (a â†’ c) â†’ (b â†’ c) â†’ (a âˆ¨ b) â†’ c
orCase f g (Inl x) = f x
orCase f g (Inr x) = g x

notNotExcludedMiddle : {P : Set} â†’ Â¬ Â¬ (P âˆ¨ (Â¬ P))
notNotExcludedMiddle notExcludedMiddle =
    let notP p = notExcludedMiddle (Inl p)
     in notExcludedMiddle (Inr notP)

-- There are various different axioms that can be added to a
-- constructive logic to get the more familiar classical logic.

proofByContradiction = {P : Set} â†’ Â¬ Â¬ P â†’ P
excludedMiddle = {P : Set} â†’ P âˆ¨ (Â¬ P)
impliesToOr = {P Q : Set} â†’ (P â†’ Q) â†’ (Â¬ P) âˆ¨ Q
-- Let's try to prove these three statements are equivalent...  you
--  may find it helpful to replace the 'doubleNegation' and others
--  with their definition in the type signatures below.
--  This is not always easy...


step1 : proofByContradiction â†’ excludedMiddle
step1 dn = dn notNotExcludedMiddle

step2 : excludedMiddle â†’ impliesToOr
step2 em pToQ = orCase (Î» p â†’ Inr (pToQ p)) Inl em

step3 : impliesToOr â†’ proofByContradiction
step3 ito {P} h =
    let excludedMiddle = ito (Î» p â†’ p)
    in orCase (Î» nP â†’ magic (h nP)) (Î» p â†’ p) excludedMiddle

-- HARDER: show that these are equivalent to Peirce's law:
peircesLaw = {P Q : Set} â†’ ((P â†’ Q) â†’ P) â†’ P

peirceToContradiction : peircesLaw â†’ proofByContradiction
peirceToContradiction pl nnP = pl (Î» nP â†’ magic (nnP nP))

excludedMiddleToPeirce : excludedMiddle â†’ peircesLaw
excludedMiddleToPeirce em pToQToP = orCase
    (Î» p â†’ p)
    (Î» nP â†’ pToQToP (Î» p â†’ magic (nP p)))
    em

----------------------
----- Exercise 9 -----
----------------------

-- Given the following data type for expressions

data Expr : Set where
  Add : Expr â†’ Expr â†’ Expr
  Val : â„• â†’ Expr

-- We can write a simple evaluator as follows
eval : Expr â†’ â„•
eval (Add l r) = eval l + eval r
eval (Val x) = x

-- We can also compile such expressions to stack machine code
-- The arguments to Cmd represent:
-- the number of elements in the input stack (modified by ADD)
-- the number of elements in the output stack (modified by PUSH and ADD)
data Cmd : (i o : â„•) â†’ Set where
  -- stop execution and return the current stack
  HALT : {i : â„•} â†’ Cmd i i
  -- push a new number on the stack
  PUSH : {i o : â„•} â†’ â„• â†’ Cmd (Succ i) o â†’ Cmd i o
  -- replace the top two elements of the stack with their sum
  ADD : {i o : â„•} â†’ Cmd (Succ i) o â†’ Cmd (Succ (Succ i)) o

Stack : â„•Â â†’ Set
Stack = Vec â„•

-- Complete the following definition, executing a list of instructions
-- Note: there 'obvious' definition is not total.  There are several
-- ways to fix this. One is to use vectors rather than lists to
-- represent stacks. To do so, however, you may also need to update
-- the Cmd datatype...

exec : {i o : â„•} â†’ Cmd i o â†’ Stack i â†’ Stack o
exec HALT xs = xs
exec (PUSH x c) xs = exec c (Cons x xs)
exec (ADD c) (Cons xâ‚€ (Cons xâ‚ xs)) = exec c (Cons (xâ‚€ + xâ‚) xs)

compile' : {i o : â„•} â†’ Cmd (Succ i) (Succ o) â†’ Expr â†’ Cmd i (Succ o)
compile' c (Add eâ‚€ eâ‚) = compile' (compile' (ADD c) eâ‚€) eâ‚
compile' c (Val x) = PUSH x c

-- Define a compiler from expresions to instructions
compile : {n : â„•} â†’ Expr â†’ Cmd n (Succ n)
compile = compile' HALT

correctness' : {i o : â„•} (c : Cmd (Succ i) (Succ o)) (e : Expr) (s : Stack i) â†’
  exec c (Cons (eval e) s) â‰¡ exec (compile' c e) s
correctness' c (Add eâ‚€ eâ‚) s =
    exec c (Cons (eval eâ‚€ + eval eâ‚) s)
    â‰¡âŸ¨ correctness' (ADD c) eâ‚€ (Cons (eval eâ‚) s) âŸ©
    exec (compile' (ADD c) eâ‚€) (Cons (eval eâ‚) s)
    â‰¡âŸ¨ correctness' (compile' (ADD c) eâ‚€) eâ‚ s âŸ©
    exec (compile' (compile' (ADD c) eâ‚€) eâ‚) s
    âˆ
correctness' c (Val x) s = Refl

-- And prove your compiler correct
correctness : {n : â„•} (e : Expr) (s : Stack n) â†’
  Cons (eval e) s â‰¡ exec (compile e) s
correctness = correctness' HALT

--BONUS exercises: extend the language with new constructs for let
--bindings, variables, new operators, mutable references, assignment,
--functions, ...
